pcuic/theories/utils/PCUICPrimitive.v
@@ -6,27 +6,30 @@ From Equations Require Import Equations.
 From Coq Require Import ssreflect.
 From Coq Require Import Uint63 SpecFloat.
 
-(** We don't enforce the type of the array here*)
-Record array_model (term : Type) :=
-  { array_instance : Instance.t;
+Record array_model {term : Type} :=
+  { array_level : Level.t;
     array_type : term;
     array_default : term;
     array_value : list term }.
 Derive NoConfusion for array_model.
+
+Arguments array_model : clear implicits.
 #[global]
 Instance array_model_eqdec {term} (e : EqDec term) : EqDec (array_model term).
 Proof. eqdec_proof. Qed.
 
+(* We use this inductive definition instead of the more direct case analysis
+  [prim_model_of] so that [prim_model] can be used in the inductive definition
+  of terms, otherwise it results in a non-strictly positive definition.
+  *)
 Inductive prim_model (term : Type) : prim_tag -> Type :=
 | primIntModel (i : PrimInt63.int) : prim_model term primInt
-| primFloatModel (f : PrimFloat.float) : prim_model term primFloat.
+| primFloatModel (f : PrimFloat.float) : prim_model term primFloat
+| primArrayModel (a : array_model term) : prim_model term primArray.
 
-(* | primIntModel (i : Int63.t) : prim_model term primInt *)
-(* | primFloatModel (f : float64_model) : prim_model term primFloat. *)
-(* | primArrayModel (a : array_model term) : prim_model term primArray. *)
 Arguments primIntModel {term}.
 Arguments primFloatModel {term}.
-(* Arguments primArrayModel {term}. *)
+Arguments primArrayModel {term}.
 
 Derive Signature NoConfusion for prim_model.
 
@@ -34,7 +37,7 @@ Definition prim_model_of (term : Type) (p : prim_tag) : Type :=
   match p with
   | primInt => PrimInt63.int
   | primFloat => PrimFloat.float
-  (* | primArray => array_model term *)
+  | primArray => array_model term
   end.
 
 Definition prim_val term := ∑ t : prim_tag, prim_model term t.
@@ -45,7 +48,7 @@ Definition prim_model_val {term} (p : prim_val term) : prim_model_of term (prim_
   match prim_val_model p in prim_model _ t return prim_model_of term t with
   | primIntModel i => i
   | primFloatModel f => f
-  (* | primArrayModel a => a *)
+  | primArrayModel a => a
   end.
 
 Lemma exist_irrel_eq {A} (P : A -> bool) (x y : sig P) : proj1_sig x = proj1_sig y -> x = y.
@@ -73,40 +76,73 @@ Qed.
 #[global]
 Instance reflect_eq_spec_float : ReflectEq SpecFloat.spec_float := EqDec_ReflectEq _.
 
-Equations eqb_prim_model {term} {t : prim_tag} (x y : prim_model term t) : bool :=
+Import ReflectEq.
+
+Definition eqb_array {term} {eqt : term -> term -> bool} (x y : array_model term) : bool :=
+   eqb x.(array_level) y.(array_level) &&
+   forallb2 eqt x.(array_value) y.(array_value) &&
+   eqt x.(array_default) y.(array_default) &&
+   eqt x.(array_type) y.(array_type).
+
+#[program,global]
+Instance reflect_eq_array {term} {req : ReflectEq term}: ReflectEq (array_model term) :=
+  { eqb := eqb_array (eqt := eqb) }.
+Next Obligation.
+  intros term req [] []; cbn. unfold eqb_array. cbn.
+  change (forallb2 eqb) with (eqb (A := list term)).
+  case: eqb_spec => //=. intros ->.
+  case: eqb_spec => //=. intros ->.
+  case: eqb_spec => //=. intros ->.
+  case: eqb_spec => //=. intros ->. constructor; auto.
+  all:constructor; congruence.
+Qed.
+
+Equations eqb_prim_model {term} {req : term -> term -> bool} {t : prim_tag} (x y : prim_model term t) : bool :=
   | primIntModel x, primIntModel y := ReflectEq.eqb x y
-  | primFloatModel x, primFloatModel y := ReflectEq.eqb x y.
+  | primFloatModel x, primFloatModel y := ReflectEq.eqb x y
+  | primArrayModel x, primArrayModel y := eqb_array (eqt:=req) x y.
 
 #[global, program]
-Instance prim_model_reflecteq {term} {p : prim_tag} : ReflectEq (prim_model term p) :=
-  {| ReflectEq.eqb := eqb_prim_model |}.
+Instance prim_model_reflecteq {term} {req : ReflectEq term} {p : prim_tag} : ReflectEq (prim_model term p) :=
+  {| ReflectEq.eqb := eqb_prim_model (req := eqb) |}.
 Next Obligation.
   intros. depelim x; depelim y; simp eqb_prim_model.
   case: ReflectEq.eqb_spec; constructor; subst; auto. congruence.
   case: ReflectEq.eqb_spec; constructor; subst; auto. congruence.
+  change (eqb_array a a0) with (eqb a a0).
+  case: ReflectEq.eqb_spec; constructor; subst; auto. congruence.
 Qed.
 
 #[global]
-Instance prim_model_eqdec {term} : forall p : prim_tag, EqDec (prim_model term p) := _.
+Instance prim_model_eqdec {term} {req : ReflectEq term} : forall p : prim_tag, EqDec (prim_model term p) := _.
 
-Equations eqb_prim_val {term} (x y : prim_val term) : bool :=
-  | (primInt; i), (primInt; i') := ReflectEq.eqb i i'
-  | (primFloat; f), (primFloat; f') := ReflectEq.eqb f f'
+Equations eqb_prim_val {term} {req : term -> term -> bool} (x y : prim_val term) : bool :=
+  | (primInt; i), (primInt; i') := eqb_prim_model (req := req) i i'
+  | (primFloat; f), (primFloat; f') := eqb_prim_model (req := req) f f'
+  | (primArray; a), (primArray; a') := eqb_prim_model (req := req) a a'
   | x, y := false.
 
 #[global, program]
-Instance prim_val_reflect_eq {term} : ReflectEq (prim_val term) :=
-  {| ReflectEq.eqb := eqb_prim_val |}.
+Instance prim_val_reflect_eq {term} {req : ReflectEq term} : ReflectEq (prim_val term) :=
+  {| ReflectEq.eqb := eqb_prim_val (req := eqb) |}.
 Next Obligation.
   intros. funelim (eqb_prim_val x y); simp eqb_prim_val.
+  change (eqb_prim_model i i') with (eqb i i').
   case: ReflectEq.eqb_spec; constructor; subst; auto. intros H; noconf H. cbn in n. auto.
   constructor. intros H; noconf H; auto.
   constructor. intros H; noconf H; auto.
+  constructor. intros H; noconf H; auto.
+  change (eqb_prim_model f f') with (eqb f f').
+  case: ReflectEq.eqb_spec; constructor; subst; auto. intros H; noconf H; auto.
+  constructor. intros H; noconf H; auto.
+  constructor. intros H; noconf H; auto.
+  constructor. intros H; noconf H; auto.
+  change (eqb_prim_model a a') with (eqb a a').
   case: ReflectEq.eqb_spec; constructor; subst; auto. intros H; noconf H; auto.
 Qed.
 
 #[global]
-Instance prim_tag_model_eqdec term : EqDec (prim_val term) := _.
+Instance prim_tag_model_eqdec term {req : ReflectEq term} : EqDec (prim_val term) := _.
 
 (** Printing *)
 
@@ -114,5 +150,5 @@ Definition string_of_prim {term} (soft : term -> string) (p : prim_val term) : s
   match p.π2 return string with
   | primIntModel f => "(int: " ^ string_of_prim_int f ^ ")"
   | primFloatModel f => "(float: " ^ string_of_float f ^ ")"
-  (* | primArrayModel a => "(array:" ^ ")" *)
+  | primArrayModel a => "(array:" ^ string_of_list soft a.(array_value) ^ ")"
   end.
